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Solver: Implementation
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a = l − r
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a = l +∼r + 1www�

Incoming Carry allows +1 for free

(l − r)[i ]⇐⇒ sum(l ,∼r , 1)[i ]
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Flattening: Comparison
(given: sz = size(l) = size(r))

Unsigned:

l < r

y
(l − r) < 0

y

Extension to sz + 1 bits

y

Perform Subtraction

y

Highest Bit is Sign

l < r ⇐⇒ carry(l ,∼r , 1)[sz ]
Signed (sign-extension instead of zero-extension):

l < r ⇐⇒ carry(l ,∼r , 1)[sz ]⊕ (l [sz − 1]⇐⇒ r [sz − 1])
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